more of iak cert

keyCert.v
@@ -5,6 +5,12 @@ Require Import Coq.Sets.Ensembles.
 
 
 
+(* Definitions *)
+(* *********** *)
+
+(* TODO: TPM and Device identities/info *)
+(* TODO: Restricted attribute for keys *)
+
 Inductive ak_val : Set :=
 | initial : ak_val
 | local : ak_val.
@@ -23,37 +29,35 @@ Inductive keyType : Type :=
 | Private : key_val -> keyType
 | Public : key_val -> keyType.
 
-(* TODO: nonce/secret *)
-(* TODO: id for tpm and device *)
+(* TODO: find better model for random numbers *)
+Definition randType := nat.
 
-(* TODO: id : id_val -> message *)
 (* TODO: hash : message -> message *)
-(* TODO: credential : message -> secret -> message *)
 Inductive message : Type :=
 | key : keyType -> message
+| rand : randType -> message
 | TPM2_Attest : keyType -> message
 | sign : message -> keyType -> message
-| credential : message -> message
+| credential : message -> randType -> message
 | encrypt : message -> keyType -> message
 | pair : message -> message -> message.
 
-(* TODO: MakeCert : keyType -> id*)
-(* TODO: TPM2_Hash : message -> command *)
-(* TODO: MakeCert : keyType -> id -> keyType -> command *)
-(* TODO: TPM2_MakeCredential : name -> secret -> keyType -> command *)
 (* TODO: CheckNonce *)
+(* TODO: TPM2_Hash : message -> command *)
 Inductive command : Type :=
 | TPM2_Create : key_val -> command
 | TPM2_Certify : keyType -> keyType -> command
 | MakeCSR : message -> message -> keyType -> command
 | TPM2_Sign : message -> keyType -> command
 | CheckSig : message -> keyType -> command
-| TPM2_MakeCredential : keyType -> keyType -> command
+| TPM2_GetRandom : randType -> command (* TODO: remove randType parameter *)
+| TPM2_MakeCredential : keyType -> randType -> keyType -> command
 | TPM2_ActivateCredential : message -> keyType -> command
 | MakeCert : keyType -> keyType -> command
 | Sequence : command -> command -> command.
 
-Definition state := Ensemble message. (* ? should be decidable ? *)
+(* corresponds to what an entity knows *)
+Definition state := Ensemble message. (* ? should be a decidable structure ? *)
 
 Notation "m1 , m2" := (pair m1 m2)  (at level 90, left associativity).
 Notation "c1 ; c2" := (Sequence c1 c2) (at level 90, left associativity).
@@ -76,22 +80,24 @@ Inductive execute : state -> command -> state -> Prop :=
     In _ st (key k) ->
     execute st (TPM2_Sign m k) (st : (sign m k))
 | E_CheckSigAK : forall st m a,
-    In _ st (sign m (Private (AK a))) -> (* ? required ? *)
+    In _ st (sign m (Private (AK a))) ->
     In _ st (key (Public (AK a))) ->
     execute st (CheckSig (sign m (Private (AK a))) (Public (AK a))) st
 | E_CheckSigCA : forall st m c,
     In _ st (sign m (Private (CA c))) -> (* ? required ? *)
     In _ st (key (Public (CA c))) ->
     execute st (CheckSig (sign m (Private (CA c))) (Public (CA c))) st
-| E_MakeCredential : forall st k k0, (* TODO: add secret credential *)
+| E_GetRandom : forall st r,
+    execute st (TPM2_GetRandom r) (st : (rand r))
+| E_MakeCredential : forall st k r k0,
     In _ st (key k) ->  (* TODO: replace with name *)
+    In _ st (rand r) ->
     In _ st (key k0) ->
-    execute st (TPM2_MakeCredential k k0) (st : (encrypt (credential (key k)) k0))
-| E_ActivateCredential : forall st m,
-    In _ st (encrypt (credential m) (Private EK)) ->
-    In _ st (key (Public EK)) ->
-    (* TODO: add secret to state *)
-    execute st (TPM2_ActivateCredential (encrypt (credential m) (Private EK)) (Public EK)) (st : (credential m))
+    execute st (TPM2_MakeCredential k r k0) (st : (encrypt (credential (key k) r) k0))
+| E_ActivateCredential : forall st m r,
+    In _ st (encrypt (credential m r) (Public EK)) ->
+    In _ st (key (Private EK)) ->
+    execute st (TPM2_ActivateCredential (encrypt (credential m r) (Public EK)) (Private EK)) (st : (credential m r) : (rand r))
 | E_MakeCert : forall st k k0,
     In _ st (key k) ->
     In _ st (key k0) ->
@@ -105,31 +111,35 @@ Inductive execute : state -> command -> state -> Prop :=
 
 
 
+(* Discovery *)
+(* ********* *)
 
-
+(* an entity who knows a message can discover additional messages from it *)
 Inductive discoverable : message -> state -> Prop :=
 | D_key : forall k,
     discoverable (key k) (Singleton _ (key k))
+| D_rand : forall r,
+    discoverable (rand r) (Singleton _ (rand r))
 | D_Attest : forall k,
     discoverable (TPM2_Attest k) (Singleton _ (TPM2_Attest k))
 | D_sign : forall m k st, 
     discoverable m st ->
     discoverable (sign m k) (st : (sign m k))
-| D_credential : forall m st,
+| D_credential : forall m r st,
     discoverable m st ->
-    discoverable (credential m) (st : (credential m))
+    discoverable (credential m r) (st : (credential m r) : (rand r))
 | D_encrypt : forall m k,
     discoverable (encrypt m k) (Singleton _ (encrypt m k))
 | D_pair : forall m1 m2 st1 st2,
     discoverable m1 st1 ->
     discoverable m2 st2 ->
     discoverable (pair m1 m2) ((Union _ st1 st2) : (m1, m2)).
-    
-(* when sending a message the recipient can discover everything in this result *)
+
+(* when sending a message the recipient can discover these additional messages *)
 Fixpoint send (m : message) : state :=
 match m with
   | sign m0 k => (send m0) : (sign m0 k)
-  | credential m0 => (send m0) : (credential m0)
+  | credential m0 r => (send m0) : (credential m0 r) : (rand r)
   | pair m1 m2 => (Union _ (send m1) (send m2)) : (m1, m2)
   | _ => Singleton _ m
 end.
@@ -170,6 +180,9 @@ Qed.
 
 
 (* Owner creation of LAK certificate based on IAK certificate *)
+(* ********************************************************** *)
+
+(* Numerical comment tags correspond to respective steps in latex documentation *)
 
 Definition ownerIni : state :=
 (*0*)(Singleton _ (key (Private (AK initial)))) :
@@ -196,6 +209,7 @@ Definition ownerFinal : state :=
 (*3*)lakCSR :
 (*4*)(sign lakCSR (Private (AK local))).
 
+(* TODO: automate the following proofs *)
 (*
 Hint Unfold In ownerIni ownerSteps lakCSR ownerFinal: core.
 Hint Resolve Union_introl Union_intror In_singleton Extensionality_Ensembles: core.
@@ -222,7 +236,7 @@ Proof.
      apply In_singleton.
 Qed.
 
-(*5*)(* send 4 *)
+(*5*)(* send (sign lakCSR (Private (AK local))) *)
 
 Definition caOwnerIni : state :=
 (*0*)(Singleton _ (key (Private (CA owner)))) :
@@ -277,11 +291,10 @@ Qed.
 
 
 
-
-
-
-
 (* OEM creation of IAK certificate based on EK certificate *)
+(* ******************************************************* *)
+
+(* Numerical comment tags correspond to respective steps in latex documentation *)
 
 Definition oemIni : state :=
 (*0*)(Singleton _ (key (Private EK))) :
@@ -306,7 +319,6 @@ Definition oemMid : state :=
 (*2*)iakCSR :
 (*3*)(sign iakCSR (Private (AK initial))).
 
-
 Theorem correct_oemMid :
 execute oemIni oemSteps1 oemMid.
 Proof.
@@ -322,23 +334,27 @@ Proof.
   -- apply Union_introl. apply Union_introl. apply Union_intror. apply In_singleton.
 Qed.
 
-(*4*)(* send 3 *)
+(*4*)(* send (sign iakCSR (Private (AK initial))) *)
 
 Definition caOemIni : state :=
 (*0*)(Singleton _ (key (Private (CA oem)))) :
      (key (Public (CA tm))).
+
+Definition r : randType := 5.
 
 Definition caOemSteps1 : command :=
 (*5*)(CheckSig (sign iakCSR (Private (AK initial)))
                (Public (AK initial))) ;
      (CheckSig (sign (key (Public EK)) (Private (CA tm)))
                (Public (CA tm))) ;
-(*6*)TPM2_MakeCredential (Public (AK initial)) (Public EK).
+(*6*)TPM2_GetRandom r ;    
+     TPM2_MakeCredential (Public (AK initial)) r (Public EK).
 
 Definition caOemMid : state :=
 (*0*)(Union _ caOemIni
 (*5*)(send (sign iakCSR (Private (AK initial))))) :
-(*6*)(encrypt (credential (key (Public (AK initial)))) (Public EK)).
+(*6*)(rand r) :
+     (encrypt (credential (key (Public (AK initial))) r) (Public EK)).
 
 Theorem correct_caOemMid :
 execute oemIni oemSteps1 oemMid /\
@@ -347,7 +363,7 @@ execute (Union _ caOemIni (send (sign iakCSR (Private (AK initial))))) caOemStep
 Proof.
   repeat try split.
   - apply correct_oemMid.
-  - unfold oemMid; unfold iakCSR. apply Union_intror. apply In_singleton.
+  - unfold oemMid. apply Union_intror. apply In_singleton.
   - unfold caOemMid; unfold caOemIni; unfold caOemSteps1; unfold iakCSR; simpl. 
     repeat eapply E_Sequence.
   -- apply E_CheckSigAK.
@@ -358,275 +374,44 @@ Proof.
   --- apply Union_intror. apply Union_introl. apply Union_introl. apply Union_introl.
       apply Union_introl. apply Union_introl. apply Union_intror. apply In_singleton.
   --- apply Union_introl. apply Union_intror. apply In_singleton.
+  -- apply E_GetRandom.
   -- apply E_MakeCredential.
-  --- apply Union_intror. apply Union_introl. apply Union_introl. apply Union_intror.
+  --- apply Union_introl. apply Union_intror. apply Union_introl. apply Union_introl.
+      apply Union_intror. apply In_singleton.
+  --- apply Union_intror. apply In_singleton.
+  --- apply Union_introl. apply Union_intror. apply Union_introl. apply Union_introl.
+      apply Union_introl. apply Union_introl. apply Union_introl. apply Union_introl.
       apply In_singleton.
-  --- apply Union_intror. apply Union_introl. apply Union_introl. apply Union_introl.
-      apply Union_introl. apply Union_introl. apply Union_introl. apply In_singleton.
 Qed.
 
-(*7*)(* send 6*)
+(*7*)(* send (encrypt (credential (key (Public (AK initial))) r) (Public EK)) *)
 
 Definition oemSteps2 : command :=
-(*8*)TPM2_ActivateCredential (encrypt (credential (key (Public (AK initial)))) (Public EK))
+(*8*)TPM2_ActivateCredential (encrypt (credential (key (Public (AK initial))) r) (Public EK))
                              (Private EK).
 
 Definition oemFinal : state :=
 (* *)(Union _ oemMid
-(*7*)(send (encrypt (credential (key (Public (AK initial)))) (Public EK)))) :
-(*8*)(credential (key (Public (AK initial)))).
+(*7*)(send (encrypt (credential (key (Public (AK initial))) r) (Public EK)))) :
+(*8*)(credential (key (Public (AK initial))) r) :
+     (rand r).
 
-
-
-
-
-
-
-
-
-
-
-
-
-(* Owner creation of LAK certificate based on IAK certificate *)
-Section CertLAK.
-
-Inductive ak_val : Set :=
-| initial : ak_val
-| local : ak_val.
-
-Inductive ca_val : Set :=
-| tm : ca_val   (* tpm manufacturer *)
-| oem : ca_val  (* original equipment manufacturer *)
-| owner : ca_val.
-
-Inductive key_val : Set :=
-| EK : key_val              (* endorsement key *)
-| AK : ak_val -> key_val    (* attestation key *)
-| CA : ca_val -> key_val.   (* certificate authority key *)
-
-Inductive keyType : Type := 
-| Private : key_val -> keyType
-| Public : key_val -> keyType.
-
-(* TODO: id for tpm and device *)
-(* TODO: nonce *)
-(* TODO: encrypt *)
-Inductive message : Type :=
-| key : keyType -> message
-| TPM2_Attest : keyType -> message
-| sign : message -> keyType -> message
-| pair : message -> message -> message.
-
-(* TODO: TPM2_Hash *)
-(* TODO: id parameter for MakeCert *)
-(* TODO: TPM2_MakeCredential *)
-(* TODO: Encrypt and TPM2_ActivateCredential *)
-(* TODO: CheckNonce *)
-Inductive command : Type :=
-| TPM2_Create : key_val -> command
-| TPM2_Certify : keyType -> keyType -> command
-| MakeCSR : message -> message -> keyType -> command
-| TPM2_Sign : message -> keyType -> command
-| CheckSig : message -> keyType -> command
-| MakeCert : keyType -> keyType -> command
-| Sequence : command -> command -> command.
-
-Definition state := Ensemble message. (* ? should be decidable ? *)
-
-Notation "m1 , m2" := (pair m1 m2)  (at level 90, left associativity).
-Notation "c1 ; c2" := (Sequence c1 c2) (at level 90, left associativity).
-Notation "A : x" := (Add message A x) (at level 90, left associativity).
-
-Inductive execute : state -> command -> state -> Prop :=
-| E_Create : forall st v, 
-    execute st (TPM2_Create v) (st : (key (Private v)) : (key (Public v)))
-| E_Certify : forall st k k0,
-    In _ st (key k) ->
-    In _ st (key k0) ->
-    execute st (TPM2_Certify k k0) (st : (sign (TPM2_Attest k) k0))
-| E_MakeCSR : forall st m1 m2 k,
-    In _ st m1 ->
-    In _ st m2 ->
-    In _ st (key k) ->
-    execute st (MakeCSR m1 m2 k) (st : m1 : m2 : (key k) : (m1, m2, (key k)))
-| E_Sign : forall st m k,
-    In _ st m ->
-    In _ st (key k) ->
-    execute st (TPM2_Sign m k) (st : (sign m k))
-| E_CheckSigAK : forall st m a,
-    In _ st m -> (* ? required ? *)
-    In _ st (key (Public (AK a))) ->
-    execute st (CheckSig (sign m (Private (AK a))) (Public (AK a))) st
-| E_CheckSigCA : forall st m c,
-    In _ st m -> (* ? required ? *)
-    In _ st (key (Public (CA c))) ->
-    execute st (CheckSig (sign m (Private (CA c))) (Public (CA c))) st
-| E_MakeCert : forall st k k0,
-    In _ st (key k) ->
-    In _ st (key k0) ->
-    execute st (MakeCert k k0) (st : (sign (key k) k0))
-| E_Sequence : forall st st' st'' c1 c2,
-    execute st c1 st' ->
-    execute st' c2 st'' ->
-    execute st (Sequence c1 c2) st''.
-
-Inductive discoverable : message -> state -> Prop :=
-| D_key : forall k,
-    discoverable (key k) (Singleton _ (key k))
-| D_Attest : forall k,
-    discoverable (TPM2_Attest k) (Singleton _ (TPM2_Attest k))
-| D_sign : forall m k st, 
-    discoverable m st ->
-    discoverable (sign m k) (st : (sign m k))
-| D_pair : forall m1 m2 st1 st2,
-    discoverable m1 st1 ->
-    discoverable m2 st2 ->
-    discoverable (pair m1 m2) ((Union _ st1 st2) : (m1, m2)).
-
-(* when sending a message the recipient can discover everything in this result *)
-Fixpoint send (m : message) : state :=
-match m with
-  | sign m0 k => (send m0) : (sign m0 k)
-  | pair m1 m2 => (Union _ (send m1) (send m2)) : (m1, m2)
-  | _ => Singleton _ m
-end.
-
-Theorem discoverableSend : forall m st,
-discoverable m st ->
-send m = st.
-Proof.
-  intros m st H; induction H; simpl; subst; reflexivity.
+Theorem correct_oemFinal :
+execute oemIni oemSteps1 oemMid /\
+In _ oemMid (sign iakCSR (Private (AK initial))) /\
+execute (Union _ caOemIni (send (sign iakCSR (Private (AK initial))))) caOemSteps1 caOemMid /\
+In _ caOemMid (encrypt (credential (key (Public (AK initial))) r) (Public EK)) /\
+execute (Union _ oemMid (send (encrypt (credential (key (Public (AK initial))) r) (Public EK)))) oemSteps2 oemFinal.
+repeat try split.
+- apply correct_caOemMid.
+- apply correct_caOemMid.
+- apply correct_caOemMid.
+- unfold caOemMid. apply Union_intror. apply In_singleton.
+- unfold oemFinal; unfold oemMid; unfold oemIni; unfold oemSteps2; unfold iakCSR; simpl.
+  apply E_ActivateCredential.
+-- apply Union_intror. apply In_singleton.
+-- apply Union_introl. apply Union_introl. apply Union_introl. apply Union_introl.
+   apply Union_introl. apply Union_introl. apply In_singleton.
 Qed.
 
-Lemma sendDiscoverable' : forall m,
-discoverable m (send m).
-Proof.
-  intros m; induction m; simpl; constructor; assumption.
-Qed.
-
-Theorem sendDiscoverable : forall m st,
-send m = st -> 
-discoverable m st.
-Proof.
-  intros m st H; induction m; subst; apply sendDiscoverable'.
-Qed.
-
-Theorem iff_DiscoverableSend : forall m st,
-discoverable m st <-> send m = st.
-Proof.
-  split.
-  - apply discoverableSend.
-  - apply sendDiscoverable.
-Qed.
-
-Definition ownerIni : state :=
-(*0*)(Singleton _ (key (Private (AK initial)))) :
-     (sign (key (Public (AK initial))) (Private (CA oem))).
-
-Definition ownerProtocol : command :=
-(*1*)TPM2_Create (AK local) ;
-(*2*)TPM2_Certify (Private (AK local)) (Private (AK initial)) ;
-(*3*)MakeCSR (sign (key (Public (AK initial))) (Private (CA oem))) 
-             (sign (TPM2_Attest (Private (AK local))) (Private (AK initial))) 
-             (Public (AK local)) ;
-(*4*)TPM2_Sign ((sign (key (Public (AK initial))) (Private (CA oem))), 
-                (sign (TPM2_Attest (Private (AK local))) (Private (AK initial))),
-                (key (Public (AK local)))) 
-               (Private (AK local)).
-
-
-Definition csrLAK : message :=
-  ((sign (key (Public (AK initial))) (Private (CA oem))),
-   (sign (TPM2_Attest (Private (AK local))) (Private (AK initial))),
-   (key (Public (AK local)))).
-
-Definition ownerFinal : state :=
-(*0*)(Singleton _ (key (Private (AK initial)))) :
-     (sign (key (Public (AK initial))) (Private (CA oem))) :
-(*1*)(key (Private (AK local))) :
-     (key (Public (AK local))) :
-(*2*)(sign (TPM2_Attest (Private (AK local))) (Private (AK initial))) :
-(*3*)(sign (key (Public (AK initial))) (Private (CA oem))) :
-     (sign (TPM2_Attest (Private (AK local))) (Private (AK initial))) :
-     (key (Public (AK local))) :
-     csrLAK :
-(*4*)(sign csrLAK (Private (AK local))).
-  
-
-Hint Unfold In ownerIni ownerProtocol csrLAK ownerFinal: core.
-Hint Resolve Union_introl Union_intror In_singleton Extensionality_Ensembles: core.
-Hint Constructors execute : core.
-
-(* auto/eauto not working *)
-Theorem ownerCertLAK_spec :
-execute ownerIni ownerProtocol ownerFinal.
-Proof.
-  unfold ownerIni; unfold ownerProtocol; unfold ownerFinal; unfold csrLAK; simpl. 
-  repeat eapply E_Sequence. 
-  - apply E_Create.
-  - apply E_Certify. 
-  -- apply Union_introl. apply Union_intror. apply In_singleton.
-  -- apply Union_introl. apply Union_introl. apply Union_introl. apply In_singleton.
-  - apply E_MakeCSR.
-  -- apply Union_introl. apply Union_introl. apply Union_introl. apply Union_intror.
-     apply In_singleton.
-  -- apply Union_intror. apply In_singleton.
-  -- apply Union_introl. apply Union_intror. apply In_singleton.
-  - apply E_Sign.
-  -- apply Union_intror. apply In_singleton.
-  -- apply Union_introl. apply Union_introl. apply Union_introl. apply Union_introl.
-     apply Union_introl. apply Union_introl. apply Union_intror. apply In_singleton.
-Qed. 
-
-(*5*)(* send 4 *)
-
-Definition caIni : state :=
-(*0*)(Singleton _ (key (Private (CA owner)))) :
-     (key (Public (CA oem))).
-
-Definition caProtocol : command :=
-(*6*)(CheckSig (sign csrLAK (Private (AK local)))
-               (Public (AK local))) ;
-     (CheckSig (sign (key (Public (AK initial))) (Private (CA oem)))
-               (Public (CA oem))) ;
-     (CheckSig (sign (TPM2_Attest (Private (AK local))) (Private (AK initial)))
-               (Public (AK initial))) ;
-(*7*)(MakeCert (Public (AK local)) (Private (CA owner))).
-
-Definition caFinal : state :=
-(*0*)(Union _ ((Singleton _ (key (Private (CA owner)))) :
-               (key (Public (CA oem))))
-(*5*)(send (sign csrLAK (Private (AK local))))) :
-(*7*)(sign (key (Public (AK local))) (Private (CA owner))). 
-
-Theorem CertLAK_spec :
-execute ownerIni ownerProtocol ownerFinal /\
-In _ ownerFinal (sign csrLAK (Private (AK local))) /\
-execute (Union _ caIni (send (sign csrLAK (Private (AK local))))) caProtocol caFinal.
-Proof.
-  repeat try split.
-  - apply ownerCertLAK_spec.
-  - unfold ownerFinal; unfold csrLAK. apply Union_intror. apply In_singleton.
-  - unfold caIni; unfold caProtocol; unfold caFinal; unfold csrLAK; simpl. 
-    repeat eapply E_Sequence.
-  -- apply E_CheckSigAK.
-  --- apply Union_intror. apply Union_introl. apply Union_intror. apply In_singleton.
-  --- apply Union_intror. apply Union_introl. apply Union_introl. apply Union_intror.
-      apply In_singleton.
-  -- apply E_CheckSigCA.
-  --- apply Union_intror. apply Union_introl. apply Union_introl. apply Union_introl.
-      apply Union_introl. apply Union_introl. apply Union_introl. apply In_singleton.
-  --- apply Union_introl. apply Union_intror. apply In_singleton.
-  -- apply E_CheckSigAK.
-  --- apply Union_intror. apply Union_introl. apply Union_introl. apply Union_introl.
-      apply Union_introl. apply Union_intror. apply Union_introl. apply In_singleton.
-  --- apply Union_intror. apply Union_introl. apply Union_introl. apply Union_introl.
-      apply Union_introl. apply Union_introl. apply Union_introl. apply In_singleton.
-  -- apply E_MakeCert.
-  --- apply Union_intror. apply Union_introl. apply Union_introl. apply Union_intror.
-      apply In_singleton.
-  --- apply Union_introl. apply Union_introl. apply In_singleton.
-Qed.
-
-End CertLAK.
+(* TODO: final OEM CA step *)
